Fix type inference by generating deep equalities for pairs

Graphiti/Core/Rewrites/PureRewrites.lean
@@ -358,6 +358,121 @@ def rewrite : Rewrite String (String × Nat) :=
 
 end Operator3
 
+namespace CondOperator1
+
+def extract_type (typ : String × Nat) : RewriteResultSL (Vector Nat 1) := do
+  unless typ.1 == "cond_operator1" do throw .done
+  return #v[typ.2]
+
+def match_node := Graphiti.match_node extract_type
+
+def matcher : Pattern String (String × Nat) 1 := fun g => do
+  throw (.error s!"{decl_name%}: not implemented")
+
+variable (T : Vector Nat 1)
+variable (M : Nat)
+
+def lhs : ExprHigh String (String × Nat) := [graph|
+    i [type = "io"];
+    o [type = "io"];
+
+    op [type = "cond_operator1", arg = $(T[0])];
+
+    i -> op [to="in1"];
+    op -> o [from="out1"];
+  ]
+
+def lhs_extract := (lhs T).extract ["op"] |>.get rfl
+theorem double_check_empty_snd : (lhs_extract T).snd = ExprHigh.mk ∅ ∅ := by rfl
+def lhsLower := (lhs_extract T).fst.lower.get rfl
+
+def rhs : ExprHigh String (String × Nat) := [graph|
+    i [type = "io"];
+    o [type = "io"];
+
+    op [type = "pure", arg = $(M+1)];
+
+    i -> op [to="in1"];
+    op -> o [from="out1"];
+  ]
+
+def rhs_extract := (rhs M).extract ["op"] |>.get rfl
+def rhsLower := (rhs_extract M).fst.lower.get rfl
+def findRhs mod := (rhs_extract 0).fst.modules.find? mod |>.map Prod.fst
+
+def rewrite : Rewrite String (String × Nat) :=
+  { abstractions := [],
+    params := 1
+    pattern := matcher,
+    rewrite := λ l n => ⟨lhsLower l, rhsLower n⟩
+    name := .some "pure-cond_operator1"
+    transformedNodes := [findRhs "op" |>.get rfl]
+    fresh_types := 1
+  }
+
+end CondOperator1
+
+namespace CondOperator2
+
+def extract_type (typ : String × Nat) : RewriteResultSL (Vector Nat 1) := do
+  unless typ.1 == "cond_operator2" do throw .done
+  return #v[typ.2]
+
+def match_node := Graphiti.match_node extract_type
+
+variable (T : Vector Nat 1)
+variable (M : Nat)
+
+def matcher : Pattern String (String × Nat) 1 := fun g => do
+  throw (.error s!"{decl_name%}: not implemented")
+
+def lhs : ExprHigh String (String × Nat) := [graph|
+    i1 [type = "io"];
+    i2 [type = "io"];
+    o [type = "io"];
+
+    op [type = "cond_operator2", arg = $(T[0])];
+
+    i1 -> op [to="in1"];
+    i2 -> op [to="in2"];
+    op -> o [from="out1"];
+  ]
+
+def lhs_extract := (lhs T).extract ["op"] |>.get rfl
+theorem double_check_empty_snd : (lhs_extract T).snd = ExprHigh.mk ∅ ∅ := by rfl
+def lhsLower := (lhs_extract T).fst.lower.get rfl
+
+def rhs : ExprHigh String (String × Nat) := [graph|
+    i1 [type = "io"];
+    i2 [type = "io"];
+    o [type = "io"];
+
+    join [type = "join", arg = $(M+1)];
+    op [type = "pure", arg = $(M+2)];
+
+    i1 -> join [to="in1"];
+    i2 -> join [to="in2"];
+    join -> op [from="out1", to="in1"];
+    op -> o [from="out1"];
+  ]
+
+def rhs_extract := (rhs M).extract ["op", "join"] |>.get rfl
+def rhsLower := (rhs_extract M).fst.lower.get rfl
+def findRhs mod := (rhs_extract 0).fst.modules.find? mod |>.map Prod.fst
+
+def rewrite : Rewrite String (String × Nat) :=
+  { abstractions := [],
+    params := 1
+    pattern := matcher,
+    rewrite := λ l n => ⟨lhsLower l, rhsLower n⟩
+    name := .some "pure-cond_operator2"
+    transformedNodes := [findRhs "op" |>.get rfl]
+    addedNodes := [findRhs "join" |>.get rfl]
+    fresh_types := 2
+  }
+
+end CondOperator2
+
 namespace Fork
 
 def extract_type (typ : String × Nat) : RewriteResultSL (Vector Nat 1) := do
@@ -451,6 +566,16 @@ def specialisedPureRewrites {n} (p : Pattern String (String × Nat) n) :=
           let (s :: _, t) ← p g | throw RewriteError.done
           Operator3.match_node s g
     }
+  , { CondOperator1.rewrite with
+        pattern := fun g => do
+          let (s :: _, t) ← p g | throw RewriteError.done
+          CondOperator1.match_node s g
+    }
+  , { CondOperator2.rewrite with
+        pattern := fun g => do
+          let (s :: _, t) ← p g | throw RewriteError.done
+          CondOperator2.match_node s g
+    }
   , { Fork.rewrite with
         pattern := fun g => do
           let (s :: _, t) ← p g | throw RewriteError.done
@@ -459,13 +584,15 @@ def specialisedPureRewrites {n} (p : Pattern String (String × Nat) n) :=
   ]
 
 def singleNodePureRewrites (s : String) :=
-  [ {Constant.rewrite with pattern := Constant.match_node s }
-  , {ConstantNat.rewrite with pattern := ConstantNat.match_node s }
-  , {ConstantBool.rewrite with pattern := ConstantBool.match_node s }
-  , {Operator1.rewrite with pattern := Operator1.match_node s }
-  , {Operator2.rewrite with pattern := Operator2.match_node s }
-  , {Operator3.rewrite with pattern := Operator3.match_node s }
-  , {Fork.rewrite with pattern := Fork.match_node s }
+  [ { Constant.rewrite with pattern := Constant.match_node s }
+  , { ConstantNat.rewrite with pattern := ConstantNat.match_node s }
+  , { ConstantBool.rewrite with pattern := ConstantBool.match_node s }
+  , { Operator1.rewrite with pattern := Operator1.match_node s }
+  , { Operator2.rewrite with pattern := Operator2.match_node s }
+  , { Operator3.rewrite with pattern := Operator3.match_node s }
+  , { CondOperator1.rewrite with pattern := Operator1.match_node s }
+  , { CondOperator2.rewrite with pattern := Operator2.match_node s }
+  , { Fork.rewrite with pattern := Fork.match_node s }
   ]
 
 def chainPureRewrites (l : List String) :=
