Graphiti/Core/WellTyped.lean
@@ -180,8 +180,7 @@ def union (t : TypeUF) (t1 t2 : TypeConstraint) : TypeUF :=
 
 def findConcrTE'' (t : TypeUF) (c : Nat) : Option TypeExpr' := do
   let (.concr n1Concr, _) :=
-      t.typeMap.toList.filter (fun val => t.ufMap.root! val.2 == t.ufMap.root! c && val.1.isConcr?)
-      |>.head?
+      t.typeMap.toList.find? (fun val => val.1.isConcr? && t.ufMap.root! val.2 == t.ufMap.root! c)
       |>.getD (.concr (.var (t.ufMap.root! c)), 0)
     | failure
   return n1Concr
@@ -206,6 +205,62 @@ def toTypeExpr (t : TypeUF) (e : TypeExpr') : Option TypeExpr := toTypeExpr' t e
 
 def findConcr' (t : TypeUF) (c : Nat) : Option TypeExpr := t.findConcrTE'' c >>= t.toTypeExpr
 def findConcr (t : TypeUF) (c : TypeConstraint) : Option TypeExpr := t.findConcrTE' c >>= t.toTypeExpr
+
+-- Egraphs would be better...
+
+def toEqMap (x : TypeUF) :=
+  x.typeMap.fold (λ m t i =>
+        m.alter (x.ufMap.root! i) (λ | none => [(i, t)] | some ts => (i, t) :: ts)
+      ) (∅ : Std.HashMap Nat (List (Nat × TypeConstraint)))
+
+instance : ToString TypeUF where
+  toString x := toString <| repr <| x.toEqMap
+
+def find_reverse {α β} [BEq α] [Hashable α] [BEq β] (s : Std.HashMap α β) (b : β) : Option α :=
+  s.toList.find? (λ x => x.2 == b) |>.map Prod.fst
+
+def addPairConstraints.once (t : TypeUF) : (TypeUF × Bool) :=
+  (t.toEqMap.fold (λ s k v =>
+    match v.find? (λ | (_, .concr (.pair _ _)) => true | _ => false) with
+    | some (_, (.concr (.pair v1 v2))) =>
+      v.foldl (λ s el =>
+       match el with
+       | (_, .concr (.pair v1' v2')) =>
+         if v1 == v1' && v2 == v2'
+         then s
+         else
+           let new_ufMap := s.1.ufMap.union! v1 v1' |>.union! v2 v2'
+           let new_typeMap := s.1.typeMap.erase (.concr (.pair v1' v2'))
+           (⟨new_typeMap, new_ufMap⟩, true)
+       | _ => s) s
+    | _ => s
+  ) (t, false))
+
+def fix_point.struct {α} (f : α → α × Bool) (e : α): Nat → α
+| 0 => e
+| n+1 => let e' := f e; if e'.2 then fix_point.struct f e'.1 n else e
+
+def fix_point {α} (f : α → α × Bool) (e : α) := fix_point.struct f e 1000
+
+def addPairConstraints (t : TypeUF) : TypeUF := fix_point addPairConstraints.once t
+
+def similarTypes (t1 t2 : TypeConstraint) : Bool :=
+  match t1, t2 with
+  | .concr (.nat), .concr (.nat) => true
+  | .concr (.bool), .concr (.bool) => true
+  | .concr (.unit), .concr (.unit) => true
+  | .concr (.tag), .concr (.tag) => true
+  /- | .concr (.var _), .concr (.var _) => true -/
+  | .concr (.pair _ _), .concr (.pair _ _) => true
+  | .concr _, .concr _ => false
+  | _, _ => true
+
+def check (t : TypeUF) : Bool :=
+  t.toEqMap.all (λ _ tc =>
+    match tc.filter (λ | (_, .concr _) => true | _ => false) with
+    | x :: y => y.map Prod.snd |>.all (similarTypes x.2)
+    | _ => true
+  )
 
 end TypeUF
 
@@ -236,11 +291,6 @@ def toTypeConstraint (sn : String × Nat) (i : String) : Except String TypeConst
     | "in1" => .ok (.uninterp "fst" (.var sn.2))
     | "in2" => .ok (.uninterp "snd" (.var sn.2))
     | _ => .error s!"could not find port: {sn}/{i}"
-  | "operator1"
-  | "operator2"
-  | "operator3"
-  | "operator4"
-  | "operator5"
   | "pure" =>
     match i with
     | "in1" => .ok (.uninterp "dom1" (.var sn.2))
@@ -255,6 +305,22 @@ def toTypeConstraint (sn : String × Nat) (i : String) : Except String TypeConst
     | "in2" | "out2" => .ok (.uninterp "snd" (.var sn.2))
     | "in1" | "out1" => .ok (.var sn.2)
     | _ => .error s!"could not find port: {sn}/{i}"
+  | "cond_operator1"
+  | "cond_operator2"
+  | "cond_operator3"
+  | "cond_operator4"
+  | "cond_operator5" =>
+    match i with
+    | "out1" => .ok (.concr .bool)
+    | _ => .ok (.concr .nat)
+  | "constantNat" =>
+    match i with
+    | "in1" => .ok (.concr .unit)
+    | _ => .ok (.concr .nat)
+  | "constantBool" =>
+    match i with
+    | "in1" => .ok (.concr .unit)
+    | _ => .ok (.concr .bool)
   | "fork2"
   | "fork3"
   | "fork4"
@@ -269,7 +335,6 @@ def toTypeConstraint (sn : String × Nat) (i : String) : Except String TypeConst
   | "merge2"
   | "sink"
   | "queue" => .ok (.var sn.2)
-  | "constantNat"
   | "mc"
   | "load"
   | "inputNat"
@@ -278,6 +343,11 @@ def toTypeConstraint (sn : String × Nat) (i : String) : Except String TypeConst
   | "outputNat2"
   | "outputNat3"
   | "outputNat4"
+  | "operator1"
+  | "operator2"
+  | "operator3"
+  | "operator4"
+  | "operator5"
   | "outputNat5" => .ok (.concr .nat)
   | "initBool"
   | "outputBool0"
@@ -285,8 +355,7 @@ def toTypeConstraint (sn : String × Nat) (i : String) : Except String TypeConst
   | "outputBool2"
   | "outputBool3"
   | "outputBool4"
-  | "outputBool5"
-  | "constantBool" => .ok (.concr .bool)
+  | "outputBool5" => .ok (.concr .bool)
   | "input"
   | "output0"
   | "output1"
@@ -314,19 +383,19 @@ def additionalConstraints (sn : String × Nat) (t : TypeUF) : TypeUF :=
     let (vfst, t1) := t.insert (.uninterp "fst" (.var sn.2))
     let (vsnd, t2) := t1.insert (.uninterp "snd" (.var sn.2))
     t2.union (.var sn.2) (.concr (.pair vfst vsnd))
-  | "operator"
-  | "pure" => t.insert (.var sn.2) |>.snd
-  | "tagger_untagger_val" =>
+  | "tag_untagger_val" =>
     let (_, t) := t.insert (.var sn.2)
-    let (_, t) := t.insert (.uninterp "snd" (.var sn.2))
+    let (vfst, t) := t.insert (.uninterp "fst" (.var sn.2))
+    let (vsnd, t) := t.insert (.uninterp "snd" (.var sn.2))
+    let t := t.union (.var sn.2) (.concr (.pair vfst vsnd))
     t.union (.uninterp "fst" (.var sn.2)) (.concr .tag)
-  | "constantNat"
-  | "load"
-  | "mc"
-  | "inputNat"
-  | "outputNat" => t.union (.var sn.2) (.concr .nat)
-  | "initBool"
-  | "constantBool" => t.union (.var sn.2) (.concr .bool)
+  /- | "constantNat"
+   - | "load"
+   - | "mc"
+   - | "inputNat"
+   - | "outputNat" => t.union (.var sn.2) (.concr .nat)
+   - | "initBool"
+   - | "constantBool" => t.union (.var sn.2) (.concr .bool) -/
   /- | "output"
    - | "input" -/
   | _ => t
@@ -337,17 +406,20 @@ def infer_equalities (e : ExprLow String (String × Nat)) (t : TypeUF) : Except 
   match e with
   | .base i e => .ok t
   | .connect c e =>
-    match findInputInst c.input e, findOutputInst c.output e, e.infer_equalities t with
-    | some inp, some out, .ok t =>
+    match findInputInst c.input e, findOutputInst c.output e with
+    | some inp, some out =>
       match inp.1.input.inverse.find? c.input, out.1.output.inverse.find? c.output with
       | some ⟨_, inpV⟩, some ⟨_, outV⟩ => do
         let tinp ← toTypeConstraint inp.2 inpV
         let tout ← toTypeConstraint out.2 outV
-        .ok (additionalConstraints inp.2 t |> additionalConstraints out.2 |>.union tinp tout)
+        let eq := additionalConstraints inp.2 t |> additionalConstraints out.2 |>.union tinp tout
+        if eq.check then
+          e.infer_equalities eq
+        else
+          .error s!"type check failed for: {out.2}/{c.output} --> {inp.2}/{c.input}\n{eq}"
       | _, _ => .error s!"could not find I/O in portmap {c.input}/{c.output}"
-    | none, _, _ => .error s!"findInputInst failed on inp: {c.input}"
-    | _, none, _ => .error s!"findOutputInst failed on inp: {c.output}"
-    | _, _, .error s => .error s
+    | none, _ => .error s!"findInputInst failed on inp: {c.input}"
+    | _, none => .error s!"findOutputInst failed on inp: {c.output}"
   | .product e1 e2 => e1.infer_equalities t >>= e2.infer_equalities
 
 def infer_types (e : ExprLow String (String × Nat)) : Except String (ExprLow String (String × TypeExpr)) := do
@@ -384,7 +456,7 @@ end WellTyped
 
 def infer_equalities (e : ExprHigh String (String × Nat)) (t : TypeUF) : Except String TypeUF := do
   let e ← ofOption' "lowering failed" e.lower_TR
-  e.infer_equalities t
+  e.infer_equalities t |>.map TypeUF.addPairConstraints
 
 def infer_types' (e : ExprHigh String (String × Nat)) : Except String (ExprHigh String (String × TypeExpr) × TypeUF) := do
   let eqs ← e.infer_equalities ⟨∅, Batteries.UnionFind.mkEmpty 100⟩
